lakefile.lean
@@ -12,6 +12,14 @@ meta if get_config? env = some "dev" then
 require «termcolor» from git
   "https://github.com/jonaprieto/lean-termcolor.git" @ "cad33339fb9e64e251840b8ad4c1a2ba4306b598"
 
+require «termcolor-layout» from git
+  "https://github.com/jonaprieto/lean-termcolor-layout.git"
+  @ "6cb5303f5ab596e6d9e8801076469c0848ddefd3"
+
+require «termcolor-widgets» from git
+  "https://github.com/jonaprieto/lean-termcolor-widgets.git"
+  @ "a0330d51b3ec3fc814e8c933fc53313a78e73724"
+
 @[default_target]
 lean_lib «TermColorTerminal» where
   globs := #[.andSubmodules `TermColorTerminal]
